code/curve25519/Hacl.EC.Ladder.fst
@@ -11,151 +11,49 @@ open Hacl.Bignum.Parameters
 open Hacl.Bignum.Limb
 open Hacl.EC.Point
 open Hacl.EC.AddAndDouble
-
+open Hacl.EC.Ladder.BigLoop
 
 module U32 = FStar.UInt32
 module H8 = Hacl.UInt8
 
 
-#set-options "--initial_fuel 0 --max_fuel 0 --z3rlimit 100"
+#reset-options "--initial_fuel 0 --max_fuel 0 --z3rlimit 10"
 
-type uint8_p = buffer H8.t
-
-private inline_for_extraction val last_bit: byt:H8.t -> Tot (b:limb{v b = 0 \/ v b = 1})
-private inline_for_extraction let last_bit byt =
-  let bit = byte_to_limb (H8.(byt >>^ 7ul)) in
-  Math.Lemmas.lemma_div_lt (H8.v byt) 8 7;
-  assert_norm(pow2 1 = 2); cut (v bit = 0 \/ v bit = 1);
-  bit
-
-private inline_for_extraction val cmult_small_loop_step:
-  nq:point ->
-  nqpq:point ->
-  nq2:point ->
-  nqpq2:point ->
-  q:point ->
-  byte:H8.t ->
-  i:ctr{U32.v i > 0} ->
-  Stack unit
-    (requires (fun h -> fmonty_pre h nq2 nqpq2 nq nqpq q))
-    (ensures (fun h0 _ h1 -> fmonty_pre h0 nq2 nqpq2 nq nqpq q
-      /\ HyperStack.modifies_one (frameOf nq) h0 h1
-      /\ fmonty_pre h1 nq nqpq nq2 nqpq2 q))
-#reset-options "--initial_fuel 0 --max_fuel 0 --z3rlimit 1000"
-private inline_for_extraction let cmult_small_loop_step nq nqpq nq2 nqpq2 q byt i =
-  let nqx = getx nq in
-  let nqz = getz nq in
-  let nqpqx = getx nqpq in
-  let nqpqz = getz nqpq in
-  let nqx2 = getx nq2 in
-  let nqz2 = getz nq2 in
-  let nqpqx2 = getx nqpq2 in
-  let nqpqz2 = getz nqpq2 in
-  let bit = last_bit byt in
-  let h0 = ST.get() in
-  swap_conditional nq nqpq bit;
-  let h1 = ST.get() in
-  lemma_reveal_modifies_2 nq nqpq h0 h1;
-  cut (fmonty_pre h1 nq2 nqpq2 nq nqpq q);
-  fmonty nq2 nqpq2 nq nqpq q;
-  let h2 = ST.get() in
-  cut (fmonty_pre h2 nq nqpq nq2 nqpq2 q);
-  swap_conditional nq2 nqpq2 bit;
-  let h3 = ST.get() in
-  lemma_reveal_modifies_2 nq nqpq h0 h1;  
-  cut (fmonty_pre h3 nq nqpq nq2 nqpq2 q)
-
-
-#reset-options "--initial_fuel 0 --max_fuel 0 --z3rlimit 1000"
-
-private val cmult_small_loop:
-  nq:point ->
-  nqpq:point ->
-  nq2:point ->
-  nqpq2:point ->
-  q:point ->
-  byte:H8.t ->
-  i:ctr{U32.v i <= 8} ->  
-  Stack unit
-    (requires (fun h -> fmonty_pre h nq2 nqpq2 nq nqpq q))
-    (ensures (fun h0 _ h1 -> fmonty_pre h0 nq2 nqpq2 nq nqpq q
-      /\ HyperStack.modifies_one (frameOf nq) h0 h1
-      /\ ((U32.v i % 2 = 1) ==> fmonty_pre h1 nq nqpq nq2 nqpq2 q)
-      /\ ((U32.v i % 2 = 0) ==> fmonty_pre h1 nq2 nqpq2 nq nqpq q)
-    ))
-#reset-options "--initial_fuel 0 --max_fuel 0 --z3rlimit 1000"
-private let rec cmult_small_loop nq nqpq nq2 nqpq2 q byt i =
-  let nqx = getx nq in
-  let nqz = getz nq in
-  let nqpqx = getx nqpq in
-  let nqpqz = getz nqpq in
-  let nqx2 = getx nq2 in
-  let nqz2 = getz nq2 in
-  let nqpqx2 = getx nqpq2 in
-  let nqpqz2 = getz nqpq2 in
-  if (U32.(i =^ 0ul)) then ()
-  else (
-    cmult_small_loop_step nq nqpq nq2 nqpq2 q byt i;
-    let t = nq in
-    let nq = nq2 in
-    let nq2 = t in
-    let t = nqpq in
-    let nqpq = nqpq2 in
-    let nqpq2 = t in
-    let byt = H8.(byt <<^ 1ul) in
-    cmult_small_loop nq nqpq nq2 nqpq2 q byt (U32.(i -^ 1ul))
-  )
-
-
-private val cmult_big_loop:
-  n:uint8_p{length n = 32} ->
-  nq:point ->
-  nqpq:point ->
-  nq2:point ->
-  nqpq2:point ->
-  q:point ->
-  i:U32.t{U32.v i <= 32} ->
-  Stack unit
-    (requires (fun h -> Buffer.live h n /\ frameOf n <> frameOf nq2 /\ fmonty_pre h nq2 nqpq2 nq nqpq q))
-    (ensures (fun h0 _ h1 -> fmonty_pre h0 nq2 nqpq2 nq nqpq q
-      /\ HyperStack.modifies_one (frameOf nq2) h0 h1
-      /\ fmonty_pre h1 nq2 nqpq2 nq nqpq q))
-#reset-options "--initial_fuel 0 --max_fuel 0 --z3rlimit 1000"      
-private let rec cmult_big_loop n nq nqpq nq2 nqpq2 q i =
-  if (U32.(i =^ 0ul)) then ()
-  else (
-    let i = U32.(i -^ 1ul) in
-    let byte = n.(i) in
-    cmult_small_loop nq nqpq nq2 nqpq2 q byte 8ul;
-    cmult_big_loop n nq nqpq nq2 nqpq2 q i
-  )
-
-
-#reset-options "--initial_fuel 0 --max_fuel 0 --z3rlimit 100"
-
-assume private val lemma_seq: n:nat{n <= 30} -> Lemma
+private val lemma_seq: #a:Type -> limb_zero:a -> n:nat{n <= 30} -> Lemma
   ((Seq.slice (Seq.slice (Seq.create 40 limb_zero) n (n+10)) 0 5 == Seq.create 5 limb_zero)
   /\ (Seq.slice (Seq.slice (Seq.create 40 limb_zero) n (n+10)) 5 10 == Seq.create 5 limb_zero))
-(* private let lemma_seq n = *)
-(*   Seq.lemma_eq_intro (Seq.slice (Seq.create 40 (limb_zero)) n (n+10)) (Seq.create 10 limb_zero); *)
-(*   Seq.lemma_eq_intro (Seq.slice (Seq.create 10 (limb_zero)) 0 (5)) (Seq.create 5 limb_zero); *)
-(*   Seq.lemma_eq_intro (Seq.slice (Seq.create 10 (limb_zero)) 5 (10)) (Seq.create 5 limb_zero) *)
+private let lemma_seq #a limb_zero n =
+  Seq.lemma_eq_intro (Seq.slice (Seq.create 40 (limb_zero)) n (n+10)) (Seq.create 10 limb_zero);
+  Seq.lemma_eq_intro (Seq.slice (Seq.create 10 (limb_zero)) 0 (5)) (Seq.create 5 limb_zero);
+  Seq.lemma_eq_intro (Seq.slice (Seq.create 10 (limb_zero)) 5 (10)) (Seq.create 5 limb_zero)
+
+private let lemma_seq2 () : Lemma (Hacl.Spec.EC.AddAndDouble.red_513 (Seq.create 5 limb_zero)) = ()
+
+val lemma_cmult__modifies: buf:buffer limb -> result:point -> h00:mem -> h0:mem -> h1:mem -> h2:mem -> Lemma
+  (requires (Buffer.live h00 buf /\ live h00 result /\ h00.tip = h0.tip /\ h0.tip = h1.tip /\ h1.tip = h2.tip
+    /\ modifies_one (frameOf buf) h0 h1 /\ modifies_1 result h1 h2 /\ frameOf buf <> frameOf result
+    /\ modifies_1 buf h00 h0))
+  (ensures (modifies (Set.union (Set.singleton (frameOf buf)) (Set.singleton (frameOf result))) h00 h2
+    /\ modifies_buf_1 (frameOf result) result h00 h2))
+#reset-options "--initial_fuel 0 --max_fuel 0 --z3rlimit 100"
+let lemma_cmult__modifies buf result h00 h0 h1 h2 =
+  lemma_reveal_modifies_1 result h1 h2;
+  lemma_reveal_modifies_1 buf h00 h0
 
 
-assume val lemma_cmult__modifies: buf:buffer limb -> result:point -> h0:mem -> h1:mem -> h2:mem -> Lemma
-  (requires (Buffer.live h0 buf /\ live h0 result
-    /\ modifies_one (frameOf buf) h0 h1 /\ modifies_1 result h1 h2 /\ frameOf buf <> frameOf result))
-  (ensures (modifies (Set.union (Set.singleton (frameOf buf)) (Set.singleton (frameOf result))) h0 h2
-    /\ modifies_buf_1 (frameOf result) result h0 h2))
-(* let lemma_cmult__modifies buf result h0 h1 h2 = *)
-(*   lemma_reveal_modifies_1 result h1 h2; *)
-(*   cut (modifies_buf_1 (frameOf result) result h1 h2); *)
-(*   cut (modifies_ref (frameOf result) !{as_ref result} h1 h2);   *)
-(*   cut (forall (i:n *)
-(*   cut (Map.sel h0.h (frameOf result) == Map.sel h1.h (frameOf result)); *)
-(*   cut (modifies_buf_1 (frameOf result) result h0 h2); *)
-(*   admit() *)
-  
+type uint8_p = Buffer.buffer H8.t
+
+
+assume private val lemma_seq': h:mem -> b:buffer limb{Buffer.live h b /\ length b = 40} -> Lemma
+  (requires (as_seq h b == Seq.create 40 limb_zero))
+  (ensures (red_513 (as_seq h (getx (Buffer.sub b 0ul 10ul)))
+    /\ red_513 (as_seq h (getz (Buffer.sub b 0ul 10ul)))))
+(* private let lemma_seq' h b = *)
+(*   let s = as_seq h b in *)
+(*   let nq = Buffer.sub b 0ul 10ul in *)
+(*   Seq.lemma_eq_intro (as_seq h nq) (Seq.create 10 limb_zero); *)
+(*   Seq.lemma_eq_intro (as_seq h (getx nq)) (Seq.create 5 limb_zero); *)
+(*   Seq.lemma_eq_intro (as_seq h (getz nq)) (Seq.create 5 limb_zero); admit() *)
 
 
 private inline_for_extraction val cmult_: result:point ->
@@ -166,32 +64,37 @@ private inline_for_extraction val cmult_: result:point ->
   (requires (fun h -> Buffer.live h scalar /\ live h q /\ live h result
     /\ Buffer.live h buf /\ frameOf buf <> frameOf q /\ frameOf buf <> frameOf scalar /\ frameOf buf <> frameOf result
     /\ as_seq h buf == Seq.create 40 limb_zero
-    /\ red_513 (as_seq h (getx q))))
+    /\ red_513 (as_seq h (getx q)) /\ red_513 (as_seq h (getz q))
+  ))
   (ensures (fun h0 _ h1 -> Buffer.live h0 scalar /\ live h0 q /\ live h0 result /\ Buffer.live h0 buf
     /\ live h1 result /\ Buffer.live h1 buf
-    (* /\ modifies_2 result buf h0 h1 *)
     /\ modifies (Set.union (Set.singleton (frameOf buf)) (Set.singleton (frameOf result))) h0 h1
     /\ modifies_buf_1 (frameOf result) result h0 h1
     /\ red_513 (as_seq h1 (getx result))
     /\ red_513 (as_seq h1 (getz result))
   ))
+#reset-options "--initial_fuel 0 --max_fuel 0 --z3rlimit 1000"
 private inline_for_extraction let cmult_ result point_buf n q =
   assert_norm(pow2 32 = 0x100000000);
-  let nq = Buffer.sub point_buf 0ul 10ul in
-  let nqpq = Buffer.sub point_buf 10ul 10ul in
-  let nq2 = Buffer.sub point_buf 20ul 10ul in
+  let nq    = Buffer.sub point_buf 0ul 10ul in
+  let nqpq  = Buffer.sub point_buf 10ul 10ul in
+  let nq2   = Buffer.sub point_buf 20ul 10ul in
   let nqpq2 = Buffer.sub point_buf 30ul 10ul in
-  lemma_seq 0; lemma_seq 10; lemma_seq 20; lemma_seq 30;
+  let h0 = ST.get() in
+  lemma_seq' h0 point_buf;
   Hacl.EC.Point.copy nqpq q;
+  let hh = ST.get() in
+  no_upd_lemma_1 h0 hh nqpq nq;
+  (getx nq).(0ul) <- limb_one;
   let h = ST.get() in
-  assume (fmonty_pre h nq2 nqpq2 nq nqpq q);
   cmult_big_loop n nq nqpq nq2 nqpq2 q 32ul;
   let h' = ST.get() in
   copy result nq;
   let h'' = ST.get() in
-  lemma_cmult__modifies point_buf result h h' h'';
-  cut (modifies_buf_1 (frameOf result) result h h'')
+  lemma_cmult__modifies point_buf result h0 h h' h''
 
+
+#reset-options "--initial_fuel 0 --max_fuel 0 --z3rlimit 100"
 
 val cmult: result:point ->
   scalar:uint8_p{length scalar = keylen} ->
@@ -206,20 +109,23 @@ val cmult: result:point ->
     /\ red_513 (as_seq h1 (getz result))
   ))
 let cmult result n q =
+  let h0 = ST.get() in
   push_frame();
   (* let nq    = result in *)
+  let h1 = ST.get() in
   let point_buf = create limb_zero 40ul in
-  (* cmult_ result point_buf n q; *)
-  let nq = Buffer.sub point_buf 0ul 10ul in
-  nq.(0ul) <- limb_one;
-  let nqpq = Buffer.sub point_buf 10ul 10ul in
-  let nq2 = Buffer.sub point_buf 20ul 10ul in
-  let nqpq2 = Buffer.sub point_buf 30ul 10ul in
-  lemma_seq 0; lemma_seq 10; lemma_seq 20; lemma_seq 30;
-  Hacl.EC.Point.copy nqpq q;
-  let h = ST.get() in
-  cut (red_513 (as_seq h (getx nq)));
-  cut (red_513 (as_seq h (getz nq)));
-  cmult_big_loop n nq nqpq nq2 nqpq2 q 32ul;
-  copy result nq;
+  (* (\* cmult_ result point_buf n q; *\) *)
+  (* let nq = Buffer.sub point_buf 0ul 10ul in *)
+  (* nq.(0ul) <- limb_one; *)
+  (* let nqpq = Buffer.sub point_buf 10ul 10ul in *)
+  (* let nq2 = Buffer.sub point_buf 20ul 10ul in *)
+  (* let nqpq2 = Buffer.sub point_buf 30ul 10ul in *)
+  (* lemma_seq 0; lemma_seq 10; lemma_seq 20; lemma_seq 30; *)
+  (* Hacl.EC.Point.copy nqpq q; *)
+  (* let h = ST.get() in *)
+  (* cut (red_513 (as_seq h (getx nq))); *)
+  (* cut (red_513 (as_seq h (getz nq))); *)
+  (* cmult_big_loop n nq nqpq nq2 nqpq2 q 32ul; *)
+  (* copy result nq; *)
+  cmult_ result point_buf n q;
   pop_frame()
