code/curve25519/Hacl.EC.Ladder.BigLoop.fst
@@ -1,0 +1,44 @@
+module Hacl.EC.Ladder.BigLoop
+
+
+open FStar.Mul
+open FStar.HyperStack
+open FStar.Ghost
+open FStar.Buffer
+
+open Hacl.Bignum.Constants
+open Hacl.Bignum.Parameters
+open Hacl.Bignum.Limb
+open Hacl.EC.Point
+open Hacl.EC.AddAndDouble
+open Hacl.EC.Ladder.SmallLoop
+
+module U32 = FStar.UInt32
+module H8 = Hacl.UInt8
+
+
+#set-options "--initial_fuel 0 --max_fuel 0 --z3rlimit 100"
+
+val cmult_big_loop:
+  n:Buffer.buffer H8.t{length n = 32} ->
+  nq:point ->
+  nqpq:point ->
+  nq2:point ->
+  nqpq2:point ->
+  q:point ->
+  i:U32.t{U32.v i <= 32} ->
+  Stack unit
+    (requires (fun h -> Buffer.live h n /\ frameOf n <> frameOf nq2 /\ fmonty_pre h nq2 nqpq2 nq nqpq q))
+    (ensures (fun h0 _ h1 -> fmonty_pre h0 nq2 nqpq2 nq nqpq q
+      /\ HyperStack.modifies_one (frameOf nq2) h0 h1
+      /\ fmonty_pre h1 nq2 nqpq2 nq nqpq q))
+#reset-options "--initial_fuel 0 --max_fuel 0 --z3rlimit 100"
+let rec cmult_big_loop n nq nqpq nq2 nqpq2 q i =
+  if (U32.(i =^ 0ul)) then ()
+  else (
+    cut (U32.v i > 0);
+    let i = U32.(i -^ 1ul) in
+    let byte = n.(i) in
+    cmult_small_loop nq nqpq nq2 nqpq2 q byte 8ul;
+    cmult_big_loop n nq nqpq nq2 nqpq2 q i
+  )
