code/curve25519/Hacl.EC.Ladder.SmallLoop.fst
@@ -1,0 +1,160 @@
+module Hacl.EC.Ladder.SmallLoop
+
+
+open FStar.Mul
+open FStar.HyperStack
+open FStar.Ghost
+open FStar.Buffer
+
+open Hacl.Bignum.Constants
+open Hacl.Bignum.Parameters
+open Hacl.Bignum.Limb
+open Hacl.EC.Point
+open Hacl.EC.AddAndDouble
+
+
+module U32 = FStar.UInt32
+module H8 = Hacl.UInt8
+
+
+#set-options "--initial_fuel 0 --max_fuel 0 --z3rlimit 100"
+
+
+type uint8_p = buffer H8.t
+
+private inline_for_extraction val last_bit: byt:H8.t -> Tot (b:limb{v b = 0 \/ v b = 1})
+private inline_for_extraction let last_bit byt =
+  let bit = byte_to_limb (H8.(byt >>^ 7ul)) in
+  Math.Lemmas.lemma_div_lt (H8.v byt) 8 7;
+  assert_norm(pow2 1 = 2); cut (v bit = 0 \/ v bit = 1);
+  bit
+
+
+private inline_for_extraction val cmult_small_loop_step_1:
+  nq:point ->
+  nqpq:point ->
+  nq2:point ->
+  nqpq2:point ->
+  q:point ->
+  byte:H8.t ->
+  i:ctr{U32.v i > 0} ->
+  Stack unit
+    (requires (fun h -> fmonty_pre h nq2 nqpq2 nq nqpq q))
+    (ensures (fun h0 _ h1 -> fmonty_pre h0 nq2 nqpq2 nq nqpq q
+      /\ HyperStack.modifies_one (frameOf nq) h0 h1
+      /\ fmonty_pre h1 nq2 nqpq2 nq nqpq q))
+#reset-options "--initial_fuel 0 --max_fuel 0 --z3rlimit 100"
+private inline_for_extraction let cmult_small_loop_step_1 nq nqpq nq2 nqpq2 q byt i =
+  let bit = last_bit byt in
+  let h0 = ST.get() in
+  swap_conditional nq nqpq bit;
+  let h1 = ST.get() in
+  lemma_reveal_modifies_2 nq nqpq h0 h1
+
+
+private inline_for_extraction val cmult_small_loop_step_2:
+  nq:point ->
+  nqpq:point ->
+  nq2:point ->
+  nqpq2:point ->
+  q:point ->
+  byte:H8.t ->
+  i:ctr{U32.v i > 0} ->
+  Stack unit
+    (requires (fun h -> fmonty_pre h nq2 nqpq2 nq nqpq q))
+    (ensures (fun h0 _ h1 -> fmonty_pre h0 nq2 nqpq2 nq nqpq q
+      /\ HyperStack.modifies_one (frameOf nq) h0 h1
+      /\ fmonty_pre h1 nq nqpq nq2 nqpq2 q))
+#reset-options "--initial_fuel 0 --max_fuel 0 --z3rlimit 100"
+private inline_for_extraction let cmult_small_loop_step_2 nq nqpq nq2 nqpq2 q byt i =
+  fmonty nq2 nqpq2 nq nqpq q
+
+
+private inline_for_extraction val cmult_small_loop_step:
+  nq:point ->
+  nqpq:point ->
+  nq2:point ->
+  nqpq2:point ->
+  q:point ->
+  byte:H8.t ->
+  i:ctr{U32.v i > 0} ->
+  Stack unit
+    (requires (fun h -> fmonty_pre h nq2 nqpq2 nq nqpq q))
+    (ensures (fun h0 _ h1 -> fmonty_pre h0 nq2 nqpq2 nq nqpq q
+      /\ HyperStack.modifies_one (frameOf nq) h0 h1
+      /\ fmonty_pre h1 nq nqpq nq2 nqpq2 q))
+#reset-options "--initial_fuel 0 --max_fuel 0 --z3rlimit 100"
+private inline_for_extraction let cmult_small_loop_step nq nqpq nq2 nqpq2 q byt i =
+  cmult_small_loop_step_1 nq nqpq nq2 nqpq2 q byt i;
+  cmult_small_loop_step_2 nq nqpq nq2 nqpq2 q byt i;
+  cmult_small_loop_step_1 nq2 nqpq2 nq nqpq q byt i
+
+
+(* private inline_for_extraction val cmult_small_loop_step: *)
+(*   nq:point -> *)
+(*   nqpq:point -> *)
+(*   nq2:point -> *)
+(*   nqpq2:point -> *)
+(*   q:point -> *)
+(*   byte:H8.t -> *)
+(*   i:ctr{U32.v i > 0} -> *)
+(*   Stack unit *)
+(*     (requires (fun h -> fmonty_pre h nq2 nqpq2 nq nqpq q)) *)
+(*     (ensures (fun h0 _ h1 -> fmonty_pre h0 nq2 nqpq2 nq nqpq q *)
+(*       /\ HyperStack.modifies_one (frameOf nq) h0 h1 *)
+(*       /\ fmonty_pre h1 nq nqpq nq2 nqpq2 q)) *)
+(* #reset-options "--initial_fuel 0 --max_fuel 0 --z3rlimit 100" *)
+(* private inline_for_extraction let cmult_small_loop_step nq nqpq nq2 nqpq2 q byt i = *)
+(*   let nqx = getx nq in *)
+(*   let nqz = getz nq in *)
+(*   let nqpqx = getx nqpq in *)
+(*   let nqpqz = getz nqpq in *)
+(*   let nqx2 = getx nq2 in *)
+(*   let nqz2 = getz nq2 in *)
+(*   let nqpqx2 = getx nqpq2 in *)
+(*   let nqpqz2 = getz nqpq2 in *)
+(*   let bit = last_bit byt in *)
+(*   let h0 = ST.get() in *)
+(*   swap_conditional nq nqpq bit; *)
+(*   let h1 = ST.get() in *)
+(*   lemma_reveal_modifies_2 nq nqpq h0 h1; *)
+(*   cut (fmonty_pre h1 nq2 nqpq2 nq nqpq q); *)
+(*   fmonty nq2 nqpq2 nq nqpq q; *)
+(*   let h2 = ST.get() in *)
+(*   cut (fmonty_pre h2 nq nqpq nq2 nqpq2 q); *)
+(*   swap_conditional nq2 nqpq2 bit; *)
+(*   let h3 = ST.get() in *)
+(*   lemma_reveal_modifies_2 nq nqpq h0 h1;   *)
+(*   cut (fmonty_pre h3 nq nqpq nq2 nqpq2 q) *)
+
+
+val cmult_small_loop:
+  nq:point ->
+  nqpq:point ->
+  nq2:point ->
+  nqpq2:point ->
+  q:point ->
+  byte:H8.t ->
+  i:ctr{U32.v i <= 8} ->  
+  Stack unit
+    (requires (fun h -> fmonty_pre h nq2 nqpq2 nq nqpq q))
+    (ensures (fun h0 _ h1 -> fmonty_pre h0 nq2 nqpq2 nq nqpq q
+      /\ HyperStack.modifies_one (frameOf nq) h0 h1
+      /\ ((U32.v i % 2 = 1) ==> fmonty_pre h1 nq nqpq nq2 nqpq2 q)
+      /\ ((U32.v i % 2 = 0) ==> fmonty_pre h1 nq2 nqpq2 nq nqpq q)
+    ))
+#reset-options "--initial_fuel 1 --max_fuel 1 --z3rlimit 1000"
+let rec cmult_small_loop nq nqpq nq2 nqpq2 q byt i =
+  if (U32.(i =^ 0ul)) then ()
+  else (
+    cut (U32.v i > 0);
+    cmult_small_loop_step nq nqpq nq2 nqpq2 q byt i;
+    let t = nq in
+    let nq = nq2 in
+    let nq2 = t in
+    let t = nqpq in
+    let nqpq = nqpq2 in
+    let nqpq2 = t in
+    let byt = H8.(byt <<^ 1ul) in
+    cmult_small_loop nq nqpq nq2 nqpq2 q byt (U32.(i -^ 1ul))
+  )
